Factoring out operators

Total/Stlc/Lang/Surface/Grammar.lean
@@ -4,20 +4,26 @@ namespace Total.Stlc.Lang.Surface
     | nat: Ty
     -- | fn (dom: List Ty) (rng: Ty): Ty
 
+  inductive UnOp: Type where
+    | not: UnOp
+
+  inductive BinOp: Type where
+    | and: BinOp
+    | or:  BinOp
+    | add: BinOp
+    | mul: BinOp
+    | eq:  BinOp
+    | neq: BinOp
+    | lt:  BinOp
+    | lte: BinOp
+    | gt:  BinOp
+    | gte: BinOp
+
   inductive Term: Type where
     | bool (b: Bool): Term
     | nat  (n: Nat): Term
-    | and (lhs rhs: Term): Term
-    | or (lhs rhs: Term): Term
-    | not (op: Term): Term
-    | add (lhs rhs: Term): Term
-    | mul (lhs rhs: Term): Term
-    | eq (lhs rhs: Term): Term
-    | neq (lhs rhs: Term): Term
-    | lt (lhs rhs: Term): Term
-    | lte (lhs rhs: Term): Term
-    | gt (lhs rhs: Term): Term
-    | gte (lhs rhs: Term): Term
+    | unOp (op: UnOp) (operand: Term): Term
+    | binOp (op: BinOp) (lhs rhs: Term): Term
     | cond (c t f: Term): Term
     -- | var  (id: String): Term
     -- | bind (id: String) (ty: Ty) (expr: Term) (scope: Term): Term
