Total/Relation.lean
@@ -8,38 +8,37 @@ namespace Relation
 end Relation
 
 inductive RTC {α: Type} (R: Relation α): Relation α where
-  | mk {x y: α}: R x y → RTC R x y
   | refl {x: α}: RTC R x x
-  | trans {x y z: α}: RTC R x y → RTC R y z → RTC R x z
+  | trans {x y z: α}: R x y → RTC R y z → RTC R x z
 
 instance {α: Type} (R: Relation α): Trans R R (RTC R) where
   trans {x y z: α}: R x y → R y z → RTC R x z
-    | hxy, hyz => .trans (.mk hxy) (.trans (.mk hyz) .refl)
+    | hxy, hyz => .trans hxy (.trans hyz .refl)
 
 instance {α: Type} (R: Relation α): Trans R (RTC R) (RTC R) where
   trans {x y z: α}: R x y → RTC R y z → RTC R x z
-    | hxy, hyz => .trans (.mk hxy) hyz
+    | hxy, hyz => .trans hxy hyz
 
--- instance {α: Type} (R: Relation α): Trans (RTC R) R (RTC R) where
---   trans hxy hyz := by
---     induction hxy with
---       | refl           => exact .trans hyz .refl
---       | trans hxy _ ih => exact .trans hxy (ih hyz)
+instance {α: Type} (R: Relation α): Trans (RTC R) R (RTC R) where
+  trans hxy hyz := by
+    induction hxy with
+      | refl           => exact .trans hyz .refl
+      | trans hxy _ ih => exact .trans hxy (ih hyz)
 
---   -- trans {x y z: α}: RTC R x y → R y z → RTC R x z
---   --   | .refl,            hyz => .trans hyz .refl
---   --   | .trans hxy' hy'y, hyz =>
---   --     have ih := trans hxy' hy'y
---   --     .trans hxy' ih
+  -- trans {x y z: α}: RTC R x y → R y z → RTC R x z
+  --   | .refl,            hyz => .trans hyz .refl
+  --   | .trans hxy' hy'y, hyz =>
+  --     have ih := trans hxy' hy'y
+  --     .trans hxy' ih
 
--- instance {α: Type} (R: Relation α): Trans (RTC R) (RTC R) (RTC R) where
---   trans hxy hyz := by
---     induction hxy with
---       | refl           => exact hyz
---       | trans hxy _ ih => exact .trans hxy (ih hyz)
+instance {α: Type} (R: Relation α): Trans (RTC R) (RTC R) (RTC R) where
+  trans hxy hyz := by
+    induction hxy with
+      | refl           => exact hyz
+      | trans hxy _ ih => exact .trans hxy (ih hyz)
 
---   -- trans {x y z: α}: RTC R x y → RTC R y z → RTC R x z
---   --     | .refl,            hyz   => hyz
---   --     | .trans hyy' hy'y, hyz   =>
---   --       have ih := trans hyy' hy'y
---   --       .trans ih hyz
+  -- trans {x y z: α}: RTC R x y → RTC R y z → RTC R x z
+  --     | .refl,            hyz   => hyz
+  --     | .trans hyy' hy'y, hyz   =>
+  --       have ih := trans hyy' hy'y
+  --       .trans ih hyz
